expression_test.v
@@ -1,8 +1,50 @@
+
+
+
 Require Import expression.
 Require Import String.
-Definition n:string := "n".
+Require Import Lia.
 
-Lemma val_test: <{val n = (5*5) ; n * 2}> -->* 50.
+
+(*NOTATION*)
+Definition x : string := "x".
+Definition y : string := "y".
+Definition z : string := "z".
+Definition n : string := "n".
+Definition fun0: string := "prod5". 
+Definition prod5: string := "prod5". 
+
+Hint Unfold x : core.
+Hint Unfold y : core.
+Hint Unfold z : core.
+
+Check <{x}>.
+Check <{fun prod5 [x:Nat] {x * 5} 5}>.
+Check <{x (fun prod5 [x:Nat] {x * 5})}>.
+Check <{val n = 25 ; n * 2}>.
+Check <{[4 >> 2][5 >> 5][6 >> 4][ > 5]}>.
+
+
+
+(*SMALL STEP SEMANTICS*)
+
+Lemma smallstep_pred_succ:forall (n:nat),<{pred (succ n)}> -->* <{n}>.
+Proof.
+intro n. eapply multi_step. apply ST_pred_step. apply ST_succ. auto.
+eapply multi_step. apply ST_pred. simpl. auto. apply multi_refl.
+Qed.
+
+(*Test of succ-pred*)
+Lemma smallstep_val:forall (n:nat),<{pred (succ n)}> -->* <{n}>.
+Proof.
+intros n0. induction n0 as [| n' Hd].
+- apply multi_step with (y := <{pred 1}>).
+  +apply ST_pred_step. apply ST_succ. reflexivity.
+  +apply multi_single. apply ST_pred. reflexivity.
+- rewrite Hd.
+
+(*Test of val*)
+Lemma smallstep_val: <{val n = (5*5) ; n * 2}> -->* 50.
 Proof.
 apply multi_step with (y := <{val n = 25 ; n * 2}>).
 apply ST_Let1. apply ST_prod. reflexivity.
@@ -11,7 +53,25 @@ apply ST_LetValue. apply v_nat.
 apply multi_single. apply ST_prod. reflexivity.
 Qed.
 
+(*Test of fun*)
+Lemma smallstep_fun: <{fun prod5 [x:Nat] {x * 5} 5}> -->* 25.
+Proof.
+apply multi_step with (y := <{5 * 5}>).
+- apply ST_AppAbs. apply v_nat.
+- apply multi_single. apply ST_prod. reflexivity.
+Qed.
 
+
+(*BIG STEP SEMANTICS*)
+
+Lemma smallstep_pred_succ:forall (n:nat),<{pred (succ n)}> -->* <{n}>.
+Proof.
+intro n. eapply multi_step. apply ST_pred_step. apply ST_succ. auto.
+eapply multi_step. apply ST_pred. simpl. auto. apply multi_refl.
+Qed.
+
+
+(*Test of val*)
 Lemma bigstep_val: <{val n = (5*5) ; n * 2}> ==> 50.
 Proof.
 apply ST_Val with (w1:=25). 
@@ -19,7 +79,6 @@ apply ST_Val with (w1:=25).
 -simpl. apply ST_Prod. reflexivity.
 Qed.
 
-Definition prod5: string := "prod5".
 Lemma bigstep_fun: <{fun prod5 [x:Nat] {x * 5} 5}> ==> 25.
 Proof.
 apply ST_Fun. simpl.
